theories/Monad.v
@@ -51,3 +51,50 @@ Module MonadNotations.
     : monad_scope.
 
 End MonadNotations.
+
+(** ** The error monad and monad transformer *)
+
+Inductive exn E A :=
+| success (x : A)
+| exception (e : E).
+
+Arguments success {E A}.
+Arguments exception {E A}.
+
+Definition exn_bind {E A B} (c : exn E A) (f : A → exn E B) :=
+  match c with
+  | success x => f x
+  | exception e => exception e
+  end.
+
+#[local] Instance MonadExn {E} : Monad (exn E) := {|
+  ret A x := success x ;
+  bind A B c f := exn_bind c f
+|}.
+
+(* Exception monad transformer *)
+#[local] Instance MonadExnT {E M} `{Monad M} : Monad (λ A, M (exn E A)) := {|
+  ret A x := ret (success x) ;
+  bind A B c f := bind (M := M) c (λ x,
+    match x with
+    | success y => f y
+    | exception e => ret (exception e)
+    end
+  )
+|}.
+
+Class MonadRaise E (M : Type → Type) := {
+  raise : ∀ (A : Type), E → M A
+}.
+
+Arguments raise {E M _ A} e.
+
+#[local] Instance MonadRaiseExnT {E M} `{Monad M} : MonadRaise E (λ A, M (exn E A)) := {|
+  raise A e := ret (exception e)
+|}.
+
+Definition succeeds {E A} (m : exn E A) :=
+  match m with
+  | success _ => true
+  | _ => false
+  end.
